compiler/src/compilerExamples/SoftmulCompile.v
@@ -1,0 +1,136 @@
+Require Import Coq.Strings.String.
+Require Import Coq.ZArith.ZArith. Local Open Scope Z_scope.
+Require Import Coq.Lists.List. Import ListNotations.
+Require Import coqutil.Word.Bitwidth32.
+Require Import riscv.Utility.MonadNotations.
+Require Import riscv.Utility.FreeMonad.
+Require Import riscv.Utility.RegisterNames.
+Require riscv.Spec.PseudoInstructions.
+Require riscv.Utility.InstructionCoercions.
+Require Import riscv.Spec.Decode.
+Require Import riscv.Spec.Machine.
+Require Import riscv.Platform.Memory.
+Require Import riscv.Spec.CSRFile.
+Require Import riscv.Utility.Utility.
+Require Import riscv.Utility.RecordSetters.
+Require Import coqutil.Decidable.
+Require Import coqutil.Z.Lia.
+Require Import coqutil.Map.Interface.
+Require Import coqutil.Tactics.Tactics.
+Require Import riscv.Utility.runsToNonDet.
+Require Import compiler.SeparationLogic.
+Require Import bedrock2.Syntax.
+Require Import bedrock2.ZnWords.
+Require Import riscv.Platform.Run.
+Require Import riscv.Utility.Encode.
+Require Import riscv.Proofs.EncodeBound.
+Require Import riscv.Platform.MinimalCSRs.
+Require Import riscv.Platform.MaterializeRiscvProgram.
+Require Import compiler.regs_initialized.
+Require Import bedrock2.SepAutoArray bedrock2.SepAuto.
+
+Section Riscv.
+  Context {word: Word.Interface.word 32}.
+  Context {word_ok: word.ok word}.
+  Context {Mem: map.map word byte}.
+  Context {Mem_ok: map.ok Mem}.
+  Context {registers: map.map Z word}.
+  Context {registers_ok: map.ok registers}.
+
+  Add Ring wring : (word.ring_theory (word := word))
+      ((*This preprocessing is too expensive to be always run, especially if
+         we do many ring_simplify in a sequence, in which case it's sufficient
+         to run it once before the ring_simplify sequence.
+         preprocess [autorewrite with rew_word_morphism],*)
+       morphism (word.ring_morph (word := word)),
+       constants [word_cst]).
+
+  (* RISC-V Monad *)
+  Local Notation M := (free riscv_primitive primitive_result).
+
+  Local Hint Mode map.map - - : typeclass_instances.
+
+  Definition instr(iset: InstructionSet)(inst: Instruction)(addr: word): Mem -> Prop :=
+    ex1 (fun z => sep (addr |-> truncated_scalar access_size.four z)
+                      (emp (decode iset z = inst /\ 0 <= z < 2 ^ 32))).
+
+  Declare Scope array_abbrevs_scope.
+  Open Scope array_abbrevs_scope.
+  Notation "'program' iset" := (array (instr iset) 4) (at level 10): array_abbrevs_scope.
+
+  (* both the finish-postcondition and the abort-postcondition are set to `post`
+     to make sure `post` holds in all cases: *)
+  Definition mcomp_sat(m: M unit)(initial: State)(post: State -> Prop): Prop :=
+    free.interpret run_primitive m initial (fun tt => post) post.
+
+  Import RegisterNames PseudoInstructions.
+  Import InstructionCoercions. Open Scope ilist_scope.
+  Import Decode.
+
+  (* a3 := a1 * a2
+     without using mul, but with a naive loop:
+     a3 := 0;
+     while (0 != a1) {
+       a3 := a3 + a2;
+       a1 := a1 - 1;
+     } *)
+  Definition softmul_insts := [[
+    Addi a3 zero 0;
+    Beq zero a1 16;
+    Add a3 a3 a2;
+    Addi a1 a1 (-1);
+    J (-12)
+  ]].
+
+  (* TODO implement in bedrock2 and compile to riscv, and also need to prove that
+     programs running on the RISC-V machine used by the compiler (without CSRs)
+     also run correctly on a RISC-V machine with CSRs and a different state type. *)
+  Definition mul_insts := [[
+    Addi t1 a1 0;
+    Srli t1 t1 5           ; (* t1 := t1 >> 5                                             *)
+    Andi s3 t1 (31*4)      ; (* s3 := i[7:12]<<2   // (rd of the MUL)*4                   *)
+    Srli t1 t1 8           ; (* t1 := t1 >> 8                                             *)
+    Andi s1 t1 (31*4)      ; (* s1 := i[15:20]<<2  // (rs1 of the MUL)*4                  *)
+    Srli t1 t1 5           ; (* t1 := t1 >> 5                                             *)
+    Andi s2 t1 (31*4)      ; (* s2 := i[20:25]<<2  // (rs2 of the MUL)*4                  *)
+    Add s1 s1 sp           ; (* s1 := s1 + stack_start                                    *)
+    Add s2 s2 sp           ; (* s2 := s2 + stack_start                                    *)
+    Add s3 s3 sp           ; (* s3 := s3 + stack_start                                    *)
+    Lw a1 s1 0             ; (* a1 := stack[s1]                                           *)
+    Lw a2 s2 0               (* a2 := stack[s2]                                           *)
+  ]] ++ softmul_insts ++ [[          (* a3 := softmul(a1,a2) *)
+    Sw s3 a3 0               (* stack[s3] := a3                *)
+  ]].
+
+  (* update if index is nonzero *)
+  Definition updNz{A: Type}(l: list A)(i: Z)(v: A): list A :=
+    if Z.eqb i 0 then l else List.upd l (Z.to_nat i) v.
+
+  Lemma mul_correct: forall initial a_regs (regvals: list word) invalidIInst R,
+      initial.(nextPc) = word.add initial.(pc) (word.of_Z 4) ->
+      map.get initial.(regs) RegisterNames.a0 = Some a_regs ->
+      map.get initial.(regs) RegisterNames.a1 = Some invalidIInst ->
+      seps [a_regs |-> word_array regvals; initial.(pc) |-> program RV32I mul_insts; R]
+           initial.(mem) ->
+      runsTo (mcomp_sat (run1 RV32I)) initial (fun final =>
+        ((* case 1: It was not the Mul instruction *)
+         (map.get final.(regs) RegisterNames.a0 = Some (word.of_Z 0) /\
+          (forall rd rs1 rs2, decode RV32IM (word.unsigned invalidIInst) <>
+                                MInstruction (Mul rd rs1 rs2)) /\
+          seps [a_regs |-> word_array regvals;
+                initial.(pc) |-> program RV32I mul_insts; R] final.(mem)) \/
+         (* case 2: It was the Mul instruction *)
+         (exists ans rd rs1 rs2 v1 v2,
+          map.get final.(regs) RegisterNames.a0 = Some ans /\
+          word.unsigned ans <> 0 /\
+          decode RV32IM (word.unsigned invalidIInst) = MInstruction (Mul rd rs1 rs2) /\
+          nth_error regvals (Z.to_nat rs1) = Some v1 /\
+          nth_error regvals (Z.to_nat rs2) = Some v2 /\
+          seps [a_regs |-> word_array (updNz regvals rd (word.mul v1 v2));
+               initial.(pc) |-> program RV32I mul_insts; R] final.(mem))) /\
+        (* In common: *)
+        final.(pc) = word.add initial.(pc) (word.mul (word.of_Z 4)
+                           (word.of_Z (Z.of_nat (List.length mul_insts)))) /\
+        final.(nextPc) = word.add final.(pc) (word.of_Z 4)).
+  Admitted.
+End Riscv.
